plugin/coq/ShouldFail.v
@@ -1,5 +1,6 @@
 Require Import List.
 Require Import Ornamental.Ornaments.
+Require Import Test.
 
 (*
  * Bellow are other kinds of changes I have tried that are not
